src/Boogie.v
@@ -1,0 +1,213 @@
+Require Import Coq.Arith.Arith.
+Require Import Coq.ZArith.ZArith.
+Require Import Pact.Lib.
+Require Import Pact.Data.MapSet.
+Require Import Coq.Classes.RelationClasses.
+
+(** Abstract syntax for the Boogie intermediate language.
+
+    This representation is dependently-typed to ensure correct construction. *)
+
+Module Boogie.
+
+Import ListNotations.
+
+Definition Id := string.
+
+Inductive Ty : Set :=
+  | TAtom : TypeAtom → Ty
+  | TMap : MapType → Ty
+  | TId : Id → TypeCtorArgs → Ty
+
+with TypeAtom : Set :=
+  | TBool
+  | TInt
+  | TReal
+
+with MapType : Set :=
+  | Mp : TypeArgs → list Ty → Ty → MapType
+
+with TypeArgs : Set :=
+  | ArgsNone : TypeArgs
+  | Args : list Id → TypeArgs
+  | ArgsAng : list Id → TypeArgs
+
+with TypeCtorArgs : Set :=
+  | CtorNone : TypeCtorArgs
+  | CtorAtom : TypeAtom → TypeCtorArgs → TypeCtorArgs
+  | CtorId : Id → TypeCtorArgs → TypeCtorArgs
+  | CtorMap : MapType → TypeCtorArgs.
+
+Definition nullaryType (n : Id) : Ty := TId n CtorNone.
+Definition noType : Ty := nullaryType "NoType"%string.
+
+Record NewType : Set := {
+  tId : Id;
+  tArgs : list Id;
+  tValue : option Ty
+}.
+
+Definition ParentEdge : Set := bool * Id.
+Definition ParentInfo : Set := option (list ParentEdge).
+
+Definition FArg : Set := option Id * Ty.
+Definition dummyFArg : Id := ""%string.
+
+Inductive UnOp : Ty → Ty → Set :=
+  | Not : UnOp (TAtom TBool) (TAtom TBool)
+  | NegI : UnOp (TAtom TInt) (TAtom TInt)
+  | NegR : UnOp (TAtom TReal) (TAtom TReal).
+
+Inductive BinOp : Ty → Ty → Ty → Set :=
+  | And     : BinOp (TAtom TBool) (TAtom TBool) (TAtom TBool)
+  | Or      : BinOp (TAtom TBool) (TAtom TBool) (TAtom TBool)
+  | Implies : BinOp (TAtom TBool) (TAtom TBool) (TAtom TBool)
+  | Explies : BinOp (TAtom TBool) (TAtom TBool) (TAtom TBool)
+  | Equiv   : BinOp (TAtom TBool) (TAtom TBool) (TAtom TBool)
+  | PlusI   : BinOp (TAtom TInt) (TAtom TInt) (TAtom TInt)
+  | MinusI  : BinOp (TAtom TInt) (TAtom TInt) (TAtom TInt)
+  | TimesI  : BinOp (TAtom TInt) (TAtom TInt) (TAtom TInt)
+  | DivI    : BinOp (TAtom TInt) (TAtom TInt) (TAtom TInt)
+  | ModI    : BinOp (TAtom TInt) (TAtom TInt) (TAtom TInt)
+  | PlusR   : BinOp (TAtom TReal) (TAtom TReal) (TAtom TReal)
+  | MinusR  : BinOp (TAtom TReal) (TAtom TReal) (TAtom TReal)
+  | TimesR  : BinOp (TAtom TReal) (TAtom TReal) (TAtom TReal)
+  | DivR    : BinOp (TAtom TReal) (TAtom TReal) (TAtom TReal)
+  | ModR    : BinOp (TAtom TReal) (TAtom TReal) (TAtom TReal)
+  | Eq {t}  : BinOp t t (TAtom TBool)
+  | Neq {t} : BinOp t t (TAtom TBool)
+  | Lc {t}  : BinOp t t (TAtom TBool) (* <: *)
+  | LsI     : BinOp (TAtom TInt) (TAtom TInt) (TAtom TBool)
+  | LeqI    : BinOp (TAtom TInt) (TAtom TInt) (TAtom TBool)
+  | GtI     : BinOp (TAtom TInt) (TAtom TInt) (TAtom TBool)
+  | GeqI    : BinOp (TAtom TInt) (TAtom TInt) (TAtom TBool)
+  | LsR     : BinOp (TAtom TReal) (TAtom TReal) (TAtom TBool)
+  | LeqR    : BinOp (TAtom TReal) (TAtom TReal) (TAtom TBool)
+  | GtR     : BinOp (TAtom TReal) (TAtom TReal) (TAtom TBool)
+  | GeqR    : BinOp (TAtom TReal) (TAtom TReal) (TAtom TBool).
+
+Inductive QOp : list Ty → Set :=
+  | Forall {ts} : QOp ts
+  | Exists {ts} : QOp ts
+  | Lambda {ts} : QOp ts.
+
+Definition IdType : Set := Id * Ty.
+
+Inductive ilist {A : Set} (B : A → Set) : list A → Set :=
+  | Nil : ilist B []
+  | Cons {t : A} {ts : list A} : B t → ilist B ts → ilist B (t :: ts).
+
+Inductive Expression : Ty → Set :=
+  | FF : Expression (TAtom TBool)
+  | TT : Expression (TAtom TBool)
+  | Numeral : N → Expression (TAtom TInt)
+  | Var {t} : Id → Expression t
+  | Application {ts t} : Id → ilist Expression ts → Expression t
+  | MapSelection {args ts t} :
+    Expression (TMap (Mp args ts t)) → ilist Expression ts → Expression t
+  | MapUpdate {args ts t} :
+    Expression (TMap (Mp args ts t)) → ilist Expression ts → Expression t →
+    Expression (TMap (Mp args ts t))
+  | Old {t} : Expression t → Expression t
+  | IfExpr {t} :
+    Expression (TAtom TBool) → Expression t → Expression t → Expression t
+  | Coercion {t} : Expression t → ∀ u : Ty, Expression u
+  | UnaryExpression {a b} :
+    UnOp a b → Expression a → Expression b
+  | BinaryExpression {a b c} :
+    BinOp a b c → Expression a → Expression b → Expression c
+  | Quantified {ts} :
+    QOp ts → ilist (λ _, Id) ts → Expression (TAtom TBool) → Expression (TAtom TBool).
+
+Record IdTypeWhere : Set := {
+  itwId : Id;
+  itwType : Ty;
+  itwWhere : Expression itwType;
+}.
+
+Definition noWhere (itw : IdTypeWhere) : IdType := (itwId itw, itwType itw).
+
+Inductive Contract : Set :=
+  | Requires : bool → Expression (TAtom TBool) → Contract
+  | Modifies : bool → list Id → Contract
+  | Ensures : bool → Expression (TAtom TBool) → Contract.
+
+Inductive SpecType : Set :=
+  | Constructors
+  | Inline
+  | Precondition
+  | Postcondition
+  | LoopInvariant
+  | Where
+  (* | Requires *)
+  (* | Modifies *)
+  (* | Ensures *)
+  | Axiom_.
+
+Record SpecClause : Set := {
+  specType : SpecType;
+  specFree : bool;
+  specExpr : Expression (TAtom TBool)
+}.
+
+Inductive WildcardExpression : Ty → Set :=
+  | Wildcard {t} : WildcardExpression t
+  | Expr {t} : Expression t → WildcardExpression t.
+
+Inductive Statement : Set :=
+  | Predicate : SpecClause → Statement
+  | Havoc : list Id → Statement
+  (** The semantics of the statements:
+
+        a[j] := E;
+        b[i][m, n] := F;
+
+      is defined as having the same semantics as:
+
+        a := a[j := E];
+        b := b[i := b[i][m, n := F]];
+
+      Since this library is only for generating Boogie code, and not for
+      parsing or representing it, the former syntax is not supported. *)
+  | Assign {ts} : ilist (λ t, Id * Expression t)%type ts → Statement
+  | Call {ts} : list Id → Id → ilist Expression ts → Statement
+  | CallForall {ts} : Id → ilist WildcardExpression ts → Statement
+  | If : WildcardExpression (TAtom TBool) → Block → option Block → Statement
+  | While : WildcardExpression (TAtom TBool) → list SpecClause → Block → Statement
+  | Break : option Id → Statement
+  | Return : Statement
+  | Goto : list Id → Statement
+  | Skip
+
+with LStatement : Set :=
+  | LS : list Id → Statement → LStatement
+
+with Block : Set :=
+  | MkBlock : list LStatement → Block.
+
+Definition singletonBlock {a a1 : Set} (s : a) : list (list a1 * a) :=
+  [([], s)].
+
+Definition Body : Set := list (list IdTypeWhere) * Block.
+
+Definition BasicBlock : Set := Id * list Statement.
+
+Definition BasicBody : Set := list IdTypeWhere * Map Id (list Statement).
+
+Inductive Decl : Set :=
+  | TypeDecl : list NewType → Decl
+  | ConstantDecl : bool → list Id → Ty → ParentInfo → bool → Decl
+  | FunctionDecl :
+    Id → list Id → list FArg → ∀ ret : FArg, option (Expression (snd ret)) → Decl
+  | AxiomDecl : Expression (TAtom TBool) → Decl
+  | VarDecl : list IdTypeWhere → Decl
+  | ProcedureDecl :
+    Id → list Id → list IdTypeWhere → list IdTypeWhere → list Contract →
+    option Body → Decl
+  | ImplementationDecl :
+    Id → list Id → list IdType → list IdType → list Body → Decl.
+
+Inductive Program : Set :=
+  | MkProgram : list Decl → Program.
+
+End Boogie.
